Begin separating implication
Signed-off-by: Sky Wilshaw <zeramorphic@proton.me>

Nominal/SepProd.lean
@@ -1,4 +1,7 @@
 import Nominal.Instances
+import Nominal.Rel
+
+open Rel
 
 /-- The *separated product* of `α` and `β` with respect to the name set `𝔸`. -/
 @[ext]
@@ -65,7 +68,7 @@ theorem supp_eq [Infinite 𝔸] [Nominal 𝔸 α] [Nominal 𝔸 β] (x : α ∗[
 # (Bi)functoriality
 -/
 
-def map [Nominal 𝔸 α] [Nominal 𝔸 β] [Nominal 𝔸 γ] [Nominal 𝔸 δ]
+def bimap [Nominal 𝔸 α] [Nominal 𝔸 β] [Nominal 𝔸 γ] [Nominal 𝔸 δ]
     (f : α → γ) (g : β → δ) (hf : Equivariant 𝔸 f) (hg : Equivariant 𝔸 g)
     (x : α ∗[𝔸] β) : γ ∗[𝔸] δ :=
   ⟨f x.fst, g x.snd, by
@@ -75,22 +78,22 @@ def map [Nominal 𝔸 α] [Nominal 𝔸 β] [Nominal 𝔸 γ] [Nominal 𝔸 δ]
     exact this a (supp_apply_subset f hf x.fst ha) b (supp_apply_subset g hg x.snd hb)⟩
 
 @[simp]
-theorem map_fst [Nominal 𝔸 α] [Nominal 𝔸 β] [Nominal 𝔸 γ] [Nominal 𝔸 δ]
+theorem bimap_fst [Nominal 𝔸 α] [Nominal 𝔸 β] [Nominal 𝔸 γ] [Nominal 𝔸 δ]
     {f : α → γ} {g : β → δ} {hf : Equivariant 𝔸 f} {hg : Equivariant 𝔸 g}
     (x : α ∗[𝔸] β) :
-    (map f g hf hg x).fst = f x.fst :=
+    (bimap f g hf hg x).fst = f x.fst :=
   rfl
 
 @[simp]
-theorem map_snd [Nominal 𝔸 α] [Nominal 𝔸 β] [Nominal 𝔸 γ] [Nominal 𝔸 δ]
+theorem bimap_snd [Nominal 𝔸 α] [Nominal 𝔸 β] [Nominal 𝔸 γ] [Nominal 𝔸 δ]
     {f : α → γ} {g : β → δ} {hf : Equivariant 𝔸 f} {hg : Equivariant 𝔸 g}
     (x : α ∗[𝔸] β) :
-    (map f g hf hg x).snd = g x.snd :=
+    (bimap f g hf hg x).snd = g x.snd :=
   rfl
 
 def first [Nominal 𝔸 α] [Nominal 𝔸 β] [Nominal 𝔸 γ]
     (f : α → γ) (hf : Equivariant 𝔸 f) : α ∗[𝔸] β → γ ∗[𝔸] β :=
-  map f id hf id_equivariant
+  bimap f id hf id_equivariant
 
 @[simp]
 theorem first_fst [Nominal 𝔸 α] [Nominal 𝔸 β] [Nominal 𝔸 γ]
@@ -106,7 +109,7 @@ theorem first_snd [Nominal 𝔸 α] [Nominal 𝔸 β] [Nominal 𝔸 γ]
 
 def second [Nominal 𝔸 α] [Nominal 𝔸 β] [Nominal 𝔸 γ]
     (f : β → γ) (hf : Equivariant 𝔸 f) : α ∗[𝔸] β → α ∗[𝔸] γ :=
-  map id f id_equivariant hf
+  bimap id f id_equivariant hf
 
 @[simp]
 theorem second_fst [Nominal 𝔸 α] [Nominal 𝔸 β] [Nominal 𝔸 γ]
@@ -229,3 +232,173 @@ def assoc [Infinite 𝔸] (α β γ : Type*) [Nominal 𝔸 α] [Nominal 𝔸 β]
   right_inv _ := rfl
 
 end SepProd
+
+/-!
+# Right adjoint
+
+Here, we define *separating implication*, the right adjoint to the functor `- ∗[𝔸] α`.
+-/
+
+/-- The *separating implication* of `α` and `β` with respect to the name set `𝔸`.
+We use the definition from section 3.4 of Nominal Sets (Pitts). -/
+@[ext]
+structure SepImp (𝔸 : Type*) [DecidableEq 𝔸] (α β : Type*) [MulPerm 𝔸 α] [MulPerm 𝔸 β] where
+  rel : α → β → Prop
+  rel_fs : FinitelySupported 𝔸 rel
+  rel_coinjective : Coinjective rel
+  mem_dom_iff x : x ∈ dom rel ↔ x #[𝔸] rel
+  mem_supp_iff a : a ∈ supp 𝔸 rel ↔ ∃ x y, rel x y ∧ a ∈ supp 𝔸 y \ supp 𝔸 x
+
+@[inherit_doc] notation:25 α " -∗["𝔸"] " β:0 => SepImp 𝔸 α β
+
+theorem Rel.Coinjective.perm {𝔸 : Type*} [DecidableEq 𝔸] {α β : Type*}
+    [MulPerm 𝔸 α] [MulPerm 𝔸 β]
+    {r : α → β → Prop} (h : Coinjective r) (π : Finperm 𝔸) :
+    Coinjective (π ⬝ r) := by
+  constructor
+  intro y₁ y₂ x h₁ h₂
+  rw [Function.perm_def, Function.perm_def, IsDiscrete.perm_eq] at h₁ h₂
+  have := h.coinjective h₁ h₂
+  rwa [perm_left_cancel_iff] at this
+
+@[simp]
+theorem Rel.dom_perm {𝔸 : Type*} [DecidableEq 𝔸] {α β : Type*}
+    [MulPerm 𝔸 α] [MulPerm 𝔸 β] (r : α → β → Prop) (π : Finperm 𝔸) :
+    dom (π ⬝ r) = (π⁻¹ ⬝ ·) ⁻¹' dom r := by
+  ext x
+  constructor
+  · rintro ⟨y, hy⟩
+    use π⁻¹ ⬝ y
+    exact hy
+  · rintro ⟨y, hy⟩
+    use π ⬝ y
+    rw [Function.perm_def, Function.perm_def, inv_perm_perm]
+    exact hy
+
+namespace SepImp
+
+variable {𝔸 : Type*} [DecidableEq 𝔸] {α β γ δ : Type*}
+
+theorem mem_dom_iff_perm [MulPerm 𝔸 α] [MulPerm 𝔸 β] {f : α -∗[𝔸] β} {π : Finperm 𝔸} (x : α) :
+    x ∈ dom (π ⬝ f.rel) ↔ x #[𝔸] (π ⬝ f.rel) := by
+  rw [dom_perm, Set.mem_preimage, fresh_perm_iff_inv_perm_fresh, f.mem_dom_iff]
+
+theorem mem_supp_iff_perm [MulPerm 𝔸 α] [MulPerm 𝔸 β] {f : α -∗[𝔸] β} {π : Finperm 𝔸} (a : 𝔸) :
+    a ∈ supp 𝔸 (π ⬝ f.rel) ↔ ∃ x y, f.rel (π⁻¹ ⬝ x) (π⁻¹ ⬝ y) ∧ a ∈ supp 𝔸 y \ supp 𝔸 x := by
+  rw [supp_perm_eq, Finset.mem_perm, f.mem_supp_iff]
+  constructor
+  · rintro ⟨x, y, h₁, h₂⟩
+    refine ⟨π ⬝ x, π ⬝ y, ?_, ?_⟩
+    · rwa [inv_perm_perm, inv_perm_perm]
+    · simp only [supp_perm_eq, Finset.mem_sdiff, Finset.mem_perm] at h₂ ⊢
+      exact h₂
+  · rintro ⟨x, y, h₁, h₂⟩
+    refine ⟨π⁻¹ ⬝ x, π⁻¹ ⬝ y, h₁, ?_⟩
+    simp only [Finset.mem_sdiff] at h₂
+    simp only [supp_perm_eq, Finperm.perm_name_eq, Finset.mem_sdiff, Finset.mem_perm,
+      _root_.inv_inv, Finperm.apply_inv_self]
+    exact h₂
+
+instance [MulPerm 𝔸 α] [MulPerm 𝔸 β] : HasPerm 𝔸 (α -∗[𝔸] β) where
+  perm π f := ⟨π ⬝ f.rel, f.rel_fs.perm π,
+    f.rel_coinjective.perm π, mem_dom_iff_perm, mem_supp_iff_perm⟩
+
+@[simp]
+theorem perm_rel [MulPerm 𝔸 α] [MulPerm 𝔸 β] (f : α -∗[𝔸] β) (π : Finperm 𝔸) :
+    (π ⬝ f).rel = π ⬝ f.rel :=
+  rfl
+
+instance [MulPerm 𝔸 α] [MulPerm 𝔸 β] : MulPerm 𝔸 (α -∗[𝔸] β) where
+  one_perm f := by
+    ext : 1
+    simp only [perm_rel, one_perm]
+  mul_perm π₁ π₂ f := by
+    ext : 1
+    simp only [perm_rel, mul_perm]
+
+@[simp]
+theorem supports_iff [MulPerm 𝔸 α] [MulPerm 𝔸 β] {f : α -∗[𝔸] β} {s : Finset 𝔸} :
+    Supports s f ↔ Supports s f.rel := by
+  simp only [Supports, SepImp.ext_iff, perm_rel]
+
+instance [Infinite 𝔸] [MulPerm 𝔸 α] [MulPerm 𝔸 β] : Nominal 𝔸 (α -∗[𝔸] β) where
+  supported f := by
+    use supp 𝔸 f.rel
+    intro π hπ
+    ext : 1
+    exact supp_supports' f.rel f.rel_fs π hπ
+
+@[simp]
+theorem supp_eq [Infinite 𝔸] [MulPerm 𝔸 α] [MulPerm 𝔸 β] (f : α -∗[𝔸] β) :
+    supp 𝔸 f = supp 𝔸 f.rel := by
+  ext a
+  simp only [Nominal.mem_supp_iff, supports_iff, mem_supp_iff' f.rel f.rel_fs]
+
+@[simp]
+theorem fresh_iff [Infinite 𝔸] [MulPerm 𝔸 α] [MulPerm 𝔸 β] (f : α -∗[𝔸] β) [MulPerm 𝔸 γ] (x : γ) :
+    x #[𝔸] f ↔ x #[𝔸] f.rel := by
+  rw [fresh_def, fresh_def, supp_eq]
+
+theorem supports_unit [Infinite 𝔸] [MulPerm 𝔸 α] [Nominal 𝔸 β] (x : β) :
+    Supports (supp 𝔸 x) (λ y (z : β ∗[𝔸] α) ↦ z.fst = x ∧ z.snd = y) := by
+  intro π hπ
+  ext y z
+  have := Nominal.supp_supports 𝔸 x π hπ
+  simp only [Function.perm_def, SepProd.perm_fst, SepProd.perm_snd, perm_left_cancel_iff,
+    IsDiscrete.perm_eq]
+  constructor
+  · rintro ⟨rfl, rfl⟩
+    rw [perm_inv_perm] at this
+    rw [← this]
+    exact ⟨rfl, rfl⟩
+  · rintro ⟨rfl, rfl⟩
+    rw [perm_eq_iff_eq_inv_perm] at this
+    rw [← this]
+    exact ⟨rfl, rfl⟩
+
+theorem unit_supp [Infinite 𝔸] [MulPerm 𝔸 α] [Nominal 𝔸 β] (x : β) :
+    IsEmpty α ∨ supp 𝔸 (λ (y : α) (z : β ∗[𝔸] α) ↦ z.fst = x ∧ z.snd = y) = supp 𝔸 x := by
+  rw [or_iff_not_imp_left, not_isEmpty_iff, Nonempty.forall]
+  intro y
+  apply subset_antisymm
+  · exact supp_minimal _ _ (supports_unit x)
+  intro a ha
+  rw [mem_supp_iff' _ ⟨_, supports_unit x⟩]
+  intro s hs
+  by_contra ha'
+  -- TODO: We need a way to make a new `y` that is fresh for `x`.
+  sorry
+
+/-- The unit of the adjunction between separated product and separating implication. -/
+def unit [Infinite 𝔸] [MulPerm 𝔸 α] [Nominal 𝔸 β] (x : β) : α -∗[𝔸] β ∗[𝔸] α where
+  rel y z := z.fst = x ∧ z.snd = y
+  rel_fs := ⟨supp 𝔸 x, supports_unit x⟩
+  rel_coinjective := by constructor; aesop
+  mem_dom_iff := sorry
+  mem_supp_iff := sorry
+
+/-- Apply a separating implication to an object.
+The result of this computation is meaningful only when `x #[𝔸] f`. -/
+noncomputable def apply [MulPerm 𝔸 α] [MulPerm 𝔸 β] (f : α -∗[𝔸] β) (x : α) [Nonempty β] : β :=
+  Classical.epsilon (λ y ↦ f.rel x y)
+
+theorem apply_spec [MulPerm 𝔸 α] [MulPerm 𝔸 β] (f : α -∗[𝔸] β) (x : α) [Nonempty β]
+    (h : x #[𝔸] f.rel) :
+    f.rel x (f.apply x) :=
+  Classical.epsilon_spec ((f.mem_dom_iff x).mpr h)
+
+theorem nonempty_of_sepProd [Infinite 𝔸] [MulPerm 𝔸 α] [MulPerm 𝔸 β]
+    (x : (α -∗[𝔸] β) ∗[𝔸] α) : Nonempty β :=
+  ⟨((x.fst.mem_dom_iff x.snd).mpr ((x.fst.fresh_iff x.snd).mp x.sep.comm)).choose⟩
+
+/-- The counit of the adjunction between separated product and separating implication. -/
+noncomputable def ev [Infinite 𝔸] [MulPerm 𝔸 α] [MulPerm 𝔸 β] (x : (α -∗[𝔸] β) ∗[𝔸] α) : β :=
+  haveI : Nonempty β := nonempty_of_sepProd x
+  x.fst.apply x.snd
+
+theorem ev_spec [Infinite 𝔸] [MulPerm 𝔸 α] [MulPerm 𝔸 β] (x : (α -∗[𝔸] β) ∗[𝔸] α) :
+    x.fst.rel x.snd (ev x) :=
+  haveI : Nonempty β := nonempty_of_sepProd x
+  apply_spec _ _ ((x.fst.fresh_iff x.snd).mp x.sep.comm)
+
+end SepImp
